theories/SLFHimpl.v
@@ -386,7 +386,7 @@ Abort.
     using the placeholder value [__] for arguments that should be instantiated
     using evars. *)
 
-Lemma xsimpl_demo_rhs_hints_skip : forall H1 (p q:loc),
+Lemma xsimpl_demo_rhs_hints_evar : forall H1 (p q:loc),
   H1 ==> \exists (n m:int), (p ~~~> n \* q ~~~> m).
 Proof using.
   intros. xsimpl __ 4.
